{
  "nbformat": 4,
  "nbformat_minor": 0,
  "metadata": {
    "colab": {
      "provenance": []
    },
    "kernelspec": {
      "name": "python3",
      "display_name": "Python 3"
    },
    "language_info": {
      "name": "python"
    }
  },
  "cells": [
    {
      "cell_type": "markdown",
      "source": [
        "#Recurssion releation in dsa"
      ],
      "metadata": {
        "id": "d9xChsM7HKdK"
      }
    },
    {
      "cell_type": "markdown",
      "source": [
        "1. Find the value of T(2) for the recurrence relation T(n) = 3T(n-1) + 12n, given that T(0)=5."
      ],
      "metadata": {
        "id": "RVfxQnzXHWZe"
      }
    },
    {
      "cell_type": "code",
      "execution_count": null,
      "metadata": {
        "id": "gm6yllSBGk7q"
      },
      "outputs": [],
      "source": [
        "'''\n",
        "Understanding the Recurrence Relation\n",
        "\n",
        "The recurrence relation T(n) = 3T(n-1) + 12n means that to find the value of the sequence at any point n, we need:\n",
        "\n",
        "(A) 3 times the value at the previous point (n-1): This is represented by 3T(n-1).\n",
        "\n",
        "(B) 12 times the current point (n): This is represented by 12n.\n",
        "\n",
        "(C) The sum of these two: This gives us the value at the current point T(n).\n",
        "\n",
        "\n",
        "\n",
        "Step by Step Solution:\n",
        "\n",
        "1. Base Case (T(0) = 5):\n",
        "This is our starting point. We are given that the sequence starts with T(0) having a value of 5.\n",
        "\n",
        "\n",
        "\n",
        "2.Finding T(1):\n",
        "\n",
        "We substitute n = 1 into the recurrence relation:\n",
        "T(1) = 3T(1-1) + 12(1)\n",
        "\n",
        "Simplifying, we get:\n",
        "T(1) = 3T(0) + 12\n",
        "\n",
        "We know that T(0) = 5, so we substitute that value:\n",
        "T(1) = 3(5) + 12\n",
        "\n",
        "Calculating, we find:\n",
        "T(1) = 15 + 12 = 27\n",
        "\n",
        "Therefore, T(1) = 27.\n",
        "\n",
        "\n",
        "\n",
        "3. Finding T(2):\n",
        "We substitute n = 2 into the recurrence relation:\n",
        "T(2) = 3T(2-1) + 12(2)\n",
        "\n",
        "Simplifying, we get:\n",
        "T(2) = 3T(1) + 24\n",
        "\n",
        "We know that T(1) = 27 (from the previous step), so we substitute that value:\n",
        "T(2) = 3(27) + 24\n",
        "\n",
        "Calculating, we find:\n",
        "T(2) = 81 + 24 = 105\n",
        "\n",
        "Therefore, T(2) = 105.\n",
        "\n",
        "'''\n",
        "\n",
        "def solve_recurrence(n):\n",
        "  \"\"\"\n",
        "  Solves the recurrence relation T(n) = 3T(n-1) + 12n with T(0) = 5.\n",
        "\n",
        "  Args:\n",
        "    n: The value for which to calculate T(n).\n",
        "\n",
        "  Returns:\n",
        "    The value of T(n).\n",
        "  \"\"\"\n",
        "  if n == 0:\n",
        "    return 5  # Base case\n",
        "  else:\n",
        "    return 3 * solve_recurrence(n - 1) + 12 * n  # Recursive step\n",
        "\n",
        "# Calculate T(2)\n",
        "result = solve_recurrence(2)\n",
        "print(f\"T(2) = {result}\")\n",
        "\n",
        "'''\n",
        "Explanation of the code\n",
        "\n",
        "Base Case: If n is 0, the function immediately returns 5, representing the base case T(0) = 5.\n",
        "\n",
        "Recursive Step: If n is not 0, the function calculates T(n) using the formula 3 * solve_recurrence(n - 1) + 12 * n.\n",
        "This part embodies the recurrence relation, where it recursively calls itself with a smaller input (n - 1) to calculate the previous term and then combines it with 12 * n to get the current term.\n",
        "\n",
        "Function Call and Output: The line result = solve_recurrence(2) calls the function to compute T(2).\n",
        "Finally, print(f\"T(2) = {result}\") displays the calculated value of T(2), which is 105.\n",
        "'''\n",
        "\n",
        "\n",
        "'''\n",
        "#Time Complexity:\n",
        "\n",
        "Finding T(2)\n",
        "\n",
        "Base Case: T(0) = 5\n",
        "\n",
        "Find T(1): Substitute n = 1 into the recurrence relation: T(1) = 3T(1-1) + 12(1) T(1) = 3T(0) + 12 T(1) = 3(5) + 12 T(1) = 15 + 12 T(1) = 27\n",
        "\n",
        "Find T(2): Substitute n = 2 into the recurrence relation: T(2) = 3T(2-1) + 12(2) T(2) = 3T(1) + 24 T(2) = 3(27) + 24 T(2) = 81 + 24 T(2) = 105\n",
        "\n",
        "Therefore, T(2) = 105\n",
        "\n",
        "Time Complexity Analysis\n",
        "\n",
        "To analyze the time complexity, let's use the iterative method or the recursion tree method. Here, I'll use the iterative method:\n",
        "\n",
        "Expand the recurrence: T(n) = 3T(n-1) + 12n = 3[3T(n-2) + 12(n-1)] + 12n = 3^2T(n-2) + 3 * 12(n-1) + 12n = 3^2[3T(n-3) + 12(n-2)] + 3 * 12(n-1) + 12n = 3^3T(n-3) + 3^2 * 12(n-2) + 3 * 12(n-1) + 12n ...\n",
        "\n",
        "Generalize: After k iterations, we have: T(n) = 3^k * T(n-k) + 12[n + 3(n-1) + 3^2(n-2) + ... + 3^(k-1)(n-(k-1))]\n",
        "\n",
        "Base Case: We want to reach the base case T(0). So, we set n-k = 0, which means k = n.\n",
        "\n",
        "Substitute k: T(n) = 3^n * T(0) + 12[n + 3(n-1) + 3^2(n-2) + ... + 3^(n-1)(1)]\n",
        "\n",
        "Simplify:\n",
        "\n",
        "The first term is 3^n * T(0) = 5 * 3^n, which is O(3^n).\n",
        "The second term is a geometric series. We can simplify it to a form that is also O(3^n).\n",
        "Therefore, the dominant term in the time complexity is O(3^n).\n",
        "\n",
        "In conclusion:\n",
        "\n",
        "T(2) = 105\n",
        "Time Complexity: O(3^n) (exponential)\n",
        "\n",
        "'''"
      ]
    },
    {
      "cell_type": "markdown",
      "source": [
        "2. Given a recurrence relation, solve it using the substitution method:\n",
        "\n",
        "a. T(n) = T(n-1) + c\n",
        "\n",
        "b. T(n) = 2T(n/2) + n\n",
        "\n",
        "c. T(n) = 2T(n/2) + c\n",
        "\n",
        "d. T(n) = T(n/2) + c"
      ],
      "metadata": {
        "id": "bDuEkec3HfGA"
      }
    },
    {
      "cell_type": "code",
      "source": [
        "'''\n",
        "a. T(n) = T(n-1) + c\n",
        "\n",
        "Solving:\n",
        "\n",
        "1. Substitute: T(n) = T(n-1) + c = [T(n-2) + c] + c = T(n-2) + 2c = [T(n-3) + c] + 2c = T(n-3) + 3c ...\n",
        "\n",
        "2. Generalize: After k substitutions, we have: T(n) = T(n-k) + kc\n",
        "\n",
        "3. Base Case: Assume T(1) = d (some constant). To reach the base case, we set n-k = 1, which means k = n-1.\n",
        "\n",
        "4. Substitute k: T(n) = T(1) + (n-1)c T(n) = d + (n-1)c\n",
        "\n",
        "5. Simplify: T(n) = cn + (d-c)\n",
        "\n",
        "Time Complexity: O(n) (linear)\n",
        "'''\n",
        "\n",
        "def solve_recurrence_a(n, c, d=0):  # Assume T(1) = d (default 0)\n",
        "  \"\"\"Solves the recurrence relation T(n) = T(n-1) + c.\"\"\"\n",
        "  if n == 1:\n",
        "    return d\n",
        "  else:\n",
        "    return solve_recurrence_a(n - 1, c, d) + c\n",
        "\n",
        "# Example usage:\n",
        "result = solve_recurrence_a(5, 2, 1)  # n=5, c=2, T(1)=1\n",
        "print(f\"T(5) = {result}\")  # Output: T(5) = 9\n",
        "\n",
        "'''\n",
        "Solving Pattern:\n",
        "This recurrence relation represents a simple loop that iterates n times, adding a constant c in each iteration.\n",
        "'''\n",
        "\n",
        "'''\n",
        "b. T(n) = 2T(n/2) + n\n",
        "\n",
        "Solving:\n",
        "\n",
        "1. Substitute: T(n) = 2T(n/2) + n = 2[2T(n/4) + n/2] + n = 4T(n/4) + 2n = 4[2T(n/8) + n/4] + 2n = 8T(n/8) + 3n ...\n",
        "\n",
        "2. Generalize: After k substitutions, we have: T(n) = 2^k * T(n/2^k) + kn\n",
        "\n",
        "3. Base Case: Assume T(1) = d. To reach the base case, we set n/2^k = 1, which means k = log₂(n).\n",
        "\n",
        "4. Substitute k: T(n) = 2^(log₂(n)) * T(1) + (log₂(n))n T(n) = n * d + n(log₂(n))\n",
        "\n",
        "5. Simplify: T(n) = n(log₂(n) + d)\n",
        "\n",
        "Time Complexity: O(n log n) (log-linear)\n",
        "'''\n",
        "import math\n",
        "\n",
        "def solve_recurrence_b(n, d=0):  # Assume T(1) = d (default 0)\n",
        "  \"\"\"Solves the recurrence relation T(n) = 2T(n/2) + n.\"\"\"\n",
        "  if n == 1:\n",
        "    return d\n",
        "  else:\n",
        "    return 2 * solve_recurrence_b(n // 2, d) + n\n",
        "\n",
        "# Example usage:\n",
        "result = solve_recurrence_b(8, 1)  # n=8, T(1)=1\n",
        "print(f\"T(8) = {result}\")  # Output: T(8) = 32\n",
        "\n",
        "'''\n",
        "Solving Pattern:\n",
        "This recurrence relation represents a divide-and-conquer algorithm where the problem is divided into two subproblems of half the size,\n",
        "and then the results are combined with a linear cost (n).\n",
        "'''\n",
        "\n",
        "'''\n",
        "c. T(n) = 2T(n/2) + c\n",
        "\n",
        "Solving: Following similar steps as in (b),\n",
        "we get: T(n) = 2^k * T(n/2^k) + kc * (2^k -1) /(2-1)\n",
        "Substitute k = log₂(n) T(n) = n * T(1) + (2^(log₂(n) )-1)c T(n) = (c+T(1))n -c\n",
        "\n",
        "Time Complexity: O(n) (linear)\n",
        "'''\n",
        "\n",
        "import math\n",
        "\n",
        "def solve_recurrence_c(n, c, d=0):  # Assume T(1) = d (default 0)\n",
        "  \"\"\"Solves the recurrence relation T(n) = 2T(n/2) + c.\"\"\"\n",
        "  if n == 1:\n",
        "    return d\n",
        "  else:\n",
        "    return 2 * solve_recurrence_c(n // 2, c, d) + c\n",
        "\n",
        "# Example usage:\n",
        "result = solve_recurrence_c(8, 2, 1)  # n=8, c=2, T(1)=1\n",
        "print(f\"T(8) = {result}\")  # Output: T(8) = 15\n",
        "'''\n",
        "Solving Pattern:\n",
        "Similar to (b), but the cost of combining subproblems is constant (c),\n",
        "resulting in linear time complexity.\n",
        "'''\n",
        "\n",
        "'''\n",
        "d. T(n) = T(n/2) + c\n",
        "\n",
        "Solving:\n",
        "\n",
        "1. Substitute: T(n) = T(n/2) + c = [T(n/4) + c] + c = T(n/4) + 2c = [T(n/8) + c] + 2c = T(n/8) + 3c ...\n",
        "\n",
        "2. Generalize: After k substitutions, we have: T(n) = T(n/2^k) + kc\n",
        "\n",
        "3. Base Case: Assume T(1) = d. To reach the base case, we set n/2^k = 1, which means k = log₂(n).\n",
        "\n",
        "4. Substitute k: T(n) = T(1) + (log₂(n))c T(n) = d + c(log₂(n))\n",
        "\n",
        "Time Complexity: O(log n) (logarithmic)\n",
        "'''\n",
        "import math\n",
        "\n",
        "def solve_recurrence_d(n, c, d=0):  # Assume T(1) = d (default 0)\n",
        "  \"\"\"Solves the recurrence relation T(n) = T(n/2) + c.\"\"\"\n",
        "  if n == 1:\n",
        "    return d\n",
        "  else:\n",
        "    return solve_recurrence_d(n // 2, c, d) + c\n",
        "\n",
        "# Example usage:\n",
        "result = solve_recurrence_d(8, 2, 1)  # n=8, c=2, T(1)=1\n",
        "print(f\"T(8) = {result}\")  # Output: T(8) = 7\n",
        "\n",
        "'''\n",
        "Solving Pattern:\n",
        "This recurrence relation represents an algorithm where the problem size is halved in each step,\n",
        "resulting in logarithmic time complexity.\n",
        "'''"
      ],
      "metadata": {
        "id": "Zg692H-_HsM1"
      },
      "execution_count": null,
      "outputs": []
    },
    {
      "cell_type": "markdown",
      "source": [
        "3. Given a recurrence relation, solve it using the recursive tree approach:\n",
        "\n",
        "a. T(n) = 2T(n-1) +1\n",
        "\n",
        "b. T(n) = 2T(n/2) + n\n"
      ],
      "metadata": {
        "id": "-XI5RSTBHslU"
      }
    },
    {
      "cell_type": "code",
      "source": [
        "'''\n",
        "a. T(n) = 2T(n-1) + 1\n",
        "\n",
        "1. Visualize the Recursion Tree:\n",
        "\n",
        "Imagine a tree where each node represents a subproblem. The root represents the original problem T(n).\n",
        "\n",
        "The root has a cost of 1 (from the \"+ 1\" in the recurrence relation).\n",
        "It has two children, representing the subproblems T(n-1). Each child also has a cost of 1.\n",
        "These children further branch into their own children (T(n-2)), and so on.\n",
        "2. Analyze the Tree Levels:\n",
        "\n",
        "Level 0 (Root): Cost = 1\n",
        "Level 1: Cost = 2 * 1 (two subproblems with cost 1 each)\n",
        "Level 2: Cost = 2^2 * 1 (four subproblems with cost 1 each)\n",
        "...\n",
        "Level k: Cost = 2^k * 1\n",
        "3. Determine Tree Height:\n",
        "\n",
        "The tree continues until we reach the base case, which is typically T(1) or T(0). In this case, the recursion stops when n - k = 1, which means k = n - 1. This is the height of the tree.\n",
        "\n",
        "4. Sum the Costs at Each Level:\n",
        "\n",
        "The total cost is the sum of the costs at each level:\n",
        "\n",
        "Total Cost = 1 + 2 + 2^2 + ... + 2^(n-1)\n",
        "\n",
        "This is a geometric series, and its sum is given by:\n",
        "\n",
        "Total Cost = (2^n - 1) / (2 - 1) = 2^n - 1\n",
        "\n",
        "5. Consider the Base Case:\n",
        "\n",
        "We need to add the cost of the base case, which we'll assume is T(1) = d. Since there are 2^(n-1) instances of the base case, the total cost for the base cases is 2^(n-1) * d.\n",
        "\n",
        "6. Final Solution:\n",
        "\n",
        "Adding the costs from the recursion and the base cases, we get:\n",
        "\n",
        "T(n) = 2^n - 1 + 2^(n-1) * d\n",
        "\n",
        "Time Complexity: O(2^n) (exponential)\n",
        "'''\n",
        "def solve_recurrence_a(n):\n",
        "  \"\"\"\n",
        "  Solves the recurrence relation T(n) = 2T(n-1) + 1 using recursion.\n",
        "  Assumes T(1) = 1 (you can change this base case if needed).\n",
        "\n",
        "  Args:\n",
        "    n: The input value for the recurrence relation.\n",
        "\n",
        "  Returns:\n",
        "    The value of T(n).\n",
        "  \"\"\"\n",
        "  if n == 1:\n",
        "    return 1  # Base case: T(1) = 1\n",
        "  else:\n",
        "    return 2 * solve_recurrence_a(n - 1) + 1\n",
        "\n",
        "# Example usage\n",
        "result = solve_recurrence_a(5)\n",
        "print(f\"T(5) = {result}\")  # Output: T(5) = 31\n",
        "\n",
        "\n",
        "'''\n",
        "b. T(n) = 2T(n/2) + n\n",
        "\n",
        "1. Visualize the Recursion Tree:\n",
        "\n",
        "The root represents T(n) and has a cost of n.\n",
        "It has two children, representing T(n/2), each with a cost of n/2.\n",
        "These children further branch into T(n/4) with costs of n/4, and so on.\n",
        "2. Analyze the Tree Levels:\n",
        "\n",
        "Level 0 (Root): Cost = n\n",
        "Level 1: Cost = 2 * (n/2) = n\n",
        "Level 2: Cost = 4 * (n/4) = n\n",
        "...\n",
        "Level k: Cost = n\n",
        "We can see that the cost at each level is n.\n",
        "\n",
        "3. Determine Tree Height:\n",
        "\n",
        "The recursion continues until we reach the base case, which is T(1). We have n/2^k = 1, which means k = log₂(n). This is the height of the tree.\n",
        "\n",
        "4. Sum the Costs at Each Level:\n",
        "\n",
        "Since the cost at each level is n and there are log₂(n) levels, the total cost is:\n",
        "\n",
        "Total Cost = n * log₂(n)\n",
        "\n",
        "5. Consider the Base Case:\n",
        "\n",
        "We need to add the cost of the base case, which we'll assume is T(1) = d. Since there are 2^(log₂(n)) = n instances of the base case, the total cost for the base cases is n * d.\n",
        "\n",
        "6. Final Solution:\n",
        "\n",
        "Adding the costs from the recursion and the base cases, we get:\n",
        "\n",
        "T(n) = n * log₂(n) + n * d\n",
        "\n",
        "Time Complexity: O(n log n) (log-linear)\n",
        "'''\n",
        "def solve_recurrence_b(n):\n",
        "  \"\"\"\n",
        "  Solves the recurrence relation T(n) = 2T(n/2) + n using recursion.\n",
        "  Assumes T(1) = 1 (you can change this base case if needed).\n",
        "\n",
        "  Args:\n",
        "    n: The input value for the recurrence relation.\n",
        "\n",
        "  Returns:\n",
        "    The value of T(n).\n",
        "  \"\"\"\n",
        "  if n == 1:\n",
        "    return 1  # Base case: T(1) = 1\n",
        "  else:\n",
        "    return 2 * solve_recurrence_b(n // 2) + n\n",
        "\n",
        "# Example usage\n",
        "result = solve_recurrence_b(8)\n",
        "print(f\"T(8) = {result}\")  # Output: T(8) = 32\n"
      ],
      "metadata": {
        "id": "AwnMdNsDHt2C"
      },
      "execution_count": null,
      "outputs": []
    }
  ]
}